examples/nsl_auth.v
@@ -134,7 +134,7 @@ Lemma public_msg1I lI lR kI kR nI :
   public (TKey Enc kR) -∗
   minted nI -∗
   □ (public nI ↔ ▷ corrupt kI kR) -∗
-  public (TEnc kR (Spec.tag (N.@"m1") (Spec.of_list [nI; TKey Enc kI]))).
+  public (TEnc (TKey Enc kR) (Spec.tag (N.@"m1") (Spec.of_list [nI; TKey Enc kI]))).
 Proof.
 iIntros "#? (#? & _ & _) #p_ekI #p_ekR #m_nI #p_nI".
 iApply public_TEncIS; eauto.
@@ -147,7 +147,7 @@ Qed.
 Lemma public_msg1E lI lR kI kR nI :
   cryptis_ctx -∗
   nsl_ctx lI lR -∗
-  public (TEnc kR (Spec.tag (N.@"m1") (Spec.of_list [nI; TKey Enc kI]))) -∗
+  public (TEnc (TKey Enc kR) (Spec.tag (N.@"m1") (Spec.of_list [nI; TKey Enc kI]))) -∗
   public (TKey Enc kR) -∗
   ▷ (minted nI ∗
      public (TKey Enc kI) ∗
@@ -176,7 +176,7 @@ Lemma public_msg2I lI lR kI kR nI nR :
   minted nR -∗
   □ (public nR ↔ ▷ corrupt kI kR) -∗
   session lR kI kR (Spec.of_list [nI; nR]) -∗
-  public (TEnc kI (Spec.tag (N.@"m2") (Spec.of_list [nI; nR; TKey Enc kR]))).
+  public (TEnc (TKey Enc kI) (Spec.tag (N.@"m2") (Spec.of_list [nI; nR; TKey Enc kR]))).
 Proof.
 iIntros "#? (_ & #? & _) #p_ekI #m_nI #p_nI #p_ekR #m_nR #p_nR #?".
 iApply public_TEncIS; eauto.
@@ -191,7 +191,8 @@ Qed.
 Lemma public_msg2E lI lR kI kR nI nR :
   cryptis_ctx -∗
   nsl_ctx lI lR -∗
-  public (TEnc kI (Spec.tag (N.@"m2") (Spec.of_list [nI; nR; TKey Enc kR]))) -∗
+  public (TEnc (TKey Enc kI)
+            (Spec.tag (N.@"m2") (Spec.of_list [nI; nR; TKey Enc kR]))) -∗
   public (TKey Enc kI) -∗
   secret kI -∗
   □ (public nI ↔ ▷ corrupt kI kR) -∗
@@ -224,7 +225,7 @@ Lemma public_msg3I lI lR kI kR nI nR :
   □ (public nR ↔ ▷ corrupt kI kR) -∗
   session lI kI kR (Spec.of_list [nI; nR]) -∗
   □ (secret kR -∗ ▷ session lR kI kR (Spec.of_list [nI; nR])) -∗
-  public (TEnc kR (Spec.tag (N.@"m3") nR)).
+  public (TEnc (TKey Enc kR) (Spec.tag (N.@"m3") nR)).
 Proof.
 iIntros "#? (_ & _ & #?) #p_ekR #m_nR #s_nR #authI #authR".
 iApply public_TEncIS; eauto.
@@ -235,7 +236,7 @@ Qed.
 Lemma public_msg3E lI lR kI kR nI nR :
   cryptis_ctx -∗
   nsl_ctx lI lR -∗
-  public (TEnc kR (Spec.tag (N.@"m3") nR)) -∗
+  public (TEnc (TKey Enc kR) (Spec.tag (N.@"m3") nR)) -∗
   secret kR -∗
   □ (public nR ↔ ▷ corrupt kI kR) -∗
   session lR kI kR (Spec.of_list [nI; nR]) -∗
